theories/tree_test.v
@@ -6,8 +6,17 @@ Definition func := b (d Func).
 Definition exp := b Exp.
 Definition build_arr := arr output prop prop.
 
+Notation r := (IP 2).
+Notation p := (IP 1).
+Notation q := (IP 0).
+Notation fail := (IP 3).
+Notation true := (IP 4).
+
+Notation tt := (IP 100).
+Notation ff := (IP 101).
+
 Definition build_progr l := {|
-  sig := [fmap].[IP false <- build_arr].[IP 1 <- build_arr].[IP 2 <- build_arr].[IP 200 <- prop];
+  sig := [fmap].[p <- build_arr].[q <- build_arr].[r <- build_arr].[true <- prop];
   rules := l;
 |}.
 
@@ -22,62 +31,31 @@ Definition matchingF (t1 t2 : Tm) (s : Sigma) := if t1 == t2 then Some s else No
 
 Definition unif : Unif := mk_Unif unify matching.
 
-Notation r := (IP 2).
-Notation p := (IP 1).
-Notation q := (IP false).
 
-Definition v_X := Tm_V (IV false).
-Definition pred_q x  := Tm_App (Tm_P p) x.
-Definition pred_p x  := Tm_App (Tm_P q) x.
-Definition pred_r x  := Tm_App (Tm_P r) x.
-Definition pred_fail := Tm_P (IP 100).
+Definition v0 := Tm_V (IV 0).
 
-Definition s1 : Sigma := [fmap].[fresh [fset IV false] <- Tm_D (ID 1)].
-Definition s2 : Sigma := [fmap].[fresh [fset IV false] <- Tm_D (ID 2)].
-Definition s3 : Sigma := empty.[fresh
-         (IV 0
-          |` (varsU_rule
-                {|
-                  head := Tm_App (Tm_P (IP 0)) (Tm_D (ID 2));
-                  premises := [::]
-                |}
-              `|` varsU_rule
-                    {|
-                      head := Tm_App (Tm_P p) (Tm_D (ID 0));
-                      premises :=
-                        [:: call (Tm_App (Tm_P (IP 0)) v_X); cut]
-                    |})) <- Tm_D (ID 1)].
-Definition pred_true := ((IP 200)).
+Notation app x y := (Tm_App x y).
 
-Definition s4 := empty.[fresh
-         (IV 0
-          |` (varsU_rule
-                {|
-                  head := Tm_App (Tm_P (IP 0)) (Tm_D (ID 2)); premises := [::]
-                |}
-              `|` varsU_rule
-                    {|
-                      head := Tm_App (Tm_P p) (Tm_D (ID 0));
-                      premises :=
-                        [:: call (Tm_App (Tm_P (IP 0)) v_X);
-                            call (Tm_P pred_true); cut]|})) <- Tm_D (ID 1)].
+Coercion Tm_P : P >-> Tm.
+
+Definition s1 : Sigma := [fmap].[fresh [fset IV 0] <- Tm_P tt].
+Definition s2 : Sigma := [fmap].[fresh [fset IV 0] <- Tm_P ff].
 
 Lemma vars_sigma_set v s: vars_sigma empty.[v <- s] = v |` vars_tm s.
 Proof. by rewrite /vars_sigma/= /codom_vars codom0_set/= !fsetU0. Qed.
 
-Definition simpl_set:= (fsetU0, fset0U, codomf0, cat0f, vars_sigma0, fsetUid, acyclic_sigma0, deref_D, deref_P, ren_P, ren_D, ren_app, deref_empty, vars_sigma_set, unify_refl, cardfs1).
+Definition simpl_set:= (fsetU0, fset0U, codomf0, cat0f, vars_sigma0, fsetUid, acyclic_sigma0, deref_P, ren_P, ren_app, deref_empty, vars_sigma_set, unify_refl, cardfs1).
 
 Section Test1.
 
   Definition p_test : program := build_progr [:: 
-      mkR (Tm_App (Tm_P p) (Tm_D (ID 1))) [::] ;
-      mkR (Tm_App (Tm_P p) (Tm_D (ID 2))) [::] ;
-      mkR (Tm_App (Tm_P r) (Tm_D (ID 2))) [::] ;
-      mkR (Tm_App (Tm_P q) (Tm_D (ID 1)))
-        [:: call (Tm_App (Tm_P p) v_X) ; call (Tm_App (Tm_P r) v_X) ] 
+      mkR (app p tt) [::] ;
+      mkR (app p ff) [::] ;
+      mkR (app r ff) [::] ;
+      mkR (app q tt) [:: call (app p v0) ; call (app r v0) ] 
     ].
 
-  Goal exists v, runT unif p_test fset0 empty (TA (call (Tm_App (Tm_P q) (Tm_D (ID 1))))) (One s2) false v.
+  Goal exists v, runT unif p_test fset0 empty (TA (call (app q tt))) (One s2) false v.
   Proof.
     repeat eexists.
     set X := [fset IV 0; fresh [fset IV 0]].
@@ -108,7 +86,6 @@ Section Test1.
       rewrite /fresh_rule/= !simpl_set.
       rewrite/rename [fresh_tm _ _ _]/= !simpl_set.
       rewrite !inE/= !simpl_set !FmapE.fmapE/=.
-      (* rewrite !simpl_set/=. *)
       rewrite in_fnd/=?inE// => JK.
       rewrite ffunE/= eqxx.
       rewrite unify_ground//=.
@@ -132,13 +109,12 @@ End Test1.
 Section Test5.
 
   Definition p_test1 : program := build_progr [:: 
-      mkR (Tm_App (Tm_P p) (Tm_D (ID false))) 
-        [::call (Tm_App (Tm_P q) v_X); cut] ;
-      mkR (Tm_App (Tm_P q) (Tm_D (ID 1))) [::] ;
-      mkR (Tm_App (Tm_P q) (Tm_D (ID 2))) [::] 
+      mkR (app p ff) [::call (app q v0); cut] ;
+      mkR (app q tt) [::] ;
+      mkR (app q ff) [::] 
     ].
 
-  Goal exists v, runT unif p_test1 fset0 empty (TA (call (Tm_App (Tm_P p) (Tm_D (ID false))))) (One s1) false v.
+  Goal exists v, runT unif p_test1 fset0 empty (TA (call (app p ff))) (One s1) false v.
   Proof.
     repeat eexists.
     apply: StepT' => //=; cycle 1.
@@ -162,14 +138,13 @@ End Test5.
 Section Test6.
 
   Definition p_test2 : program := build_progr [:: 
-      mkR ((Tm_P pred_true)) [::];
-      mkR (Tm_App (Tm_P p) (Tm_D (ID false))) 
-        [::call (Tm_App (Tm_P q) v_X);call ((Tm_P pred_true)); cut] ;
-      mkR (Tm_App (Tm_P q) (Tm_D (ID 1))) [::] ;
-      mkR (Tm_App (Tm_P q) (Tm_D (ID 2))) [::] 
+      mkR true [::];
+      mkR (app p tt) [::call (app q v0); call true; cut] ;
+      mkR (app q tt) [::] ;
+      mkR (app q ff) [::] 
   ].
 
-  Goal exists r, runT unif p_test2 fset0 empty (TA (call (Tm_App (Tm_P p) (Tm_D (ID false)))) ) (One s1) false r.
+  Goal exists r, runT unif p_test2 fset0 empty (TA (call (app p tt)) ) (One s1) false r.
   Proof.
     repeat eexists.
     apply: StepT' => //; cycle 1.
@@ -226,17 +201,13 @@ Section Test2.
 End Test2.
 
 Section map.
-  Definition map := IP 0.
-  Definition cons := ID 0.
-  Definition nil := ID 1.
-  Definition one := ID 2.
-  Definition two := ID 3.
-  Definition four := ID 5.
-  Definition double := IP 4.
-
-  Coercion Tm_P : P >-> Tm. 
-  Coercion Tm_D : D >-> Tm. 
-  Coercion Tm_V : V >-> Tm. 
+  Definition cons := IP 501.
+  Definition nil := IP 502.
+  Definition one := IP 503.
+  Definition two := IP 504.
+  Definition four := IP 505.
+  Definition map := IP 600.
+  Definition double := IP 601.
 
   Definition mapS := arr input (arr input exp (arr output exp func)) (arr input exp (arr output exp func)).
   Definition consS := arr output exp exp.
@@ -246,27 +217,28 @@ Section map.
   Definition fourS := exp.
   Definition doubleS := arr input exp func.
 
-  Definition X := IV 1.
-  Definition X' := IV 10.
-  Definition Y := IV 2.
-  Definition Y' := IV 20.
-  Definition F := IV 3.
+  Definition X := IV 300.
+  Definition X' := IV 301.
+  Definition Y := IV 400.
+  Definition Y' := IV 401.
+  Definition F := IV 500.
 
+  Coercion Tm_V : V >-> Tm.
 
   Definition p' := {|
     sig := [fmap].[map <- mapS].[double <- doubleS];
     rules := 
-      mkR (Tm_App (Tm_App (Tm_App map F) nil) nil) [::] ::
-      mkR (Tm_App (Tm_App (Tm_App map F) (Tm_App (Tm_App cons X) Y)) (Tm_App (Tm_App cons X') Y') ) 
-        [:: call (Tm_App (Tm_App F X) X'); call (Tm_App (Tm_App (Tm_App map F) Y) Y')] ::
-      mkR (Tm_App (Tm_App double one) two) [::]
+      mkR (app (app (app map F) nil) nil) [::] ::
+      mkR (app (app (app map F) (app (app cons X) Y)) (app (app cons X') Y') ) 
+        [:: call (app (app F X) X'); call (app (app (app map F) Y) Y')] ::
+      mkR (app (app double one) two) [::]
       :: [::]
   |}.
 
-  Definition list12 := Tm_App (Tm_App cons one) nil.
-  Definition list24 := Tm_App (Tm_App cons two) nil.
+  Definition list12 := app (app cons one) nil.
+  Definition list24 := app (app cons two) nil.
 
-  Definition map12d := Tm_App (Tm_App (Tm_App map double) list12) X.
+  Definition map12d := app (app (app map double) list12) X.
 
   (* Lemma get_input_vars_ground m T:
     all ground T -> get_input_vars m T = fset0.
@@ -287,8 +259,7 @@ Section map.
   Lemma fstS T1 T2 (a:T1) (b:T2): (a,b).1 = a. by []. Qed.
   Lemma sndS T1 T2 (a:T1) (b:T2): (a,b).2 = b. by []. Qed.
 
-  (*
-  Lemma select_cons m ft md x xs s: select u m ft md (x::xs) s = 
+  (* Lemma select_cons m ft md x xs s: select u m ft md (x::xs) s = 
     (if inl m != get_tm_hd (head x)
       then select u m ft md xs s
       else
@@ -299,40 +270,56 @@ Section map.
       (vars_sigma sigma1 `|` varsU_rule x `|` fv, (sigma1, premises x) :: rs)
       | None => select u m ft md xs s
       end).
-  Proof. by []. Qed.
+  Proof. by []. Qed. *)
 
-  Lemma select_consF m ft md x xs s:
-    inl m = get_tm_hd (head x) ->
-    select u m ft md (x::xs) s = 
-    match H u (get_input_vars md ft) md ft (flatten_term (head x)) s with
-    | Some sigma1 =>
-      let '(fv, rs) := select u m ft md xs s in
-      (vars_sigma sigma1 `|` varsU_rule x `|` fv, (sigma1, premises x) :: rs)
-    | None => select u m ft md xs s
+  Lemma select_consF sP ft x xs s:
+    (* inl m = get_tm_hd (head x) -> *)
+    select u sP ft (x::xs) s = 
+    match H u sP (get_input_vars sP ft).1 ft (head x) s with
+    | Some (_, sigma1) =>
+      let '(fv, rs) := select u sP ft xs s in
+      (vars_sigma sigma1 `|` varsU_rule x `|` fv, ((sigma1, premises x) :: rs))
+    | None => select u sP ft xs s
     end.
-  Proof. by move=> /=->; rewrite eqxx. Qed.
-
+  Proof. by rewrite//=. Qed.
 
   Lemma inl_map_get_tm_hdmap:
     inl map == get_tm_hd map.
   Proof. by []. Qed.
 
-  Lemma ifTS T (a b:T) : (if true then a else b) = a. by []. Qed.
-  Lemma ifFS T (a b:T) : (if false then a else b) = b. by []. Qed.
+  (* Lemma ifTS T (a b:T) : (if true then a else b) = a. by []. Qed.
+  Lemma ifFS T (a b:T) : (if false then a else b) = b. by []. Qed. *)
   Lemma fmapIn e (S: {fset V}) (f: V) (H : e \in S):
     [ffun x : S => f].[? e] = Some f.
   Proof. by rewrite in_fnd/= ffunE/=. Qed.
 
-  Lemma fresh_tm_app s m f a: fresh_tm s m (Tm_App f a) = 
+  Lemma fresh_tm_app s m f a: fresh_tm s m (app f a) = 
     ((fresh_tm (fresh_tm s m f).1 (fresh_tm s m f).2 a)).
   Proof. by rewrite/=!push -surjective_pairing. Qed.
 
   Lemma fresh_tm_P s r p: fresh_tm s r (Tm_P p) = (s, r). by []. Qed.
-  Lemma fresh_tm_D s r p: fresh_tm s r (Tm_D p) = (s, r). by []. Qed.
-  Lemma getfmap12d: (get_input_vars [:: input;  input;  output] (flatten_term map12d)) = fset0.
-  Proof. by rewrite/= !simpl_set. Qed.
+  (* Lemma getfmap12d: (get_input_vars [:: input;  input;  output] (flatten_term map12d)) = fset0.
+  Proof. by rewrite/= !simpl_set. Qed. *)
 
     (* Print fresh_tm. *)
+
+  Lemma get_input_vars_map12d:
+    (get_input_vars p' map12d).1 = fset0.
+  Proof.
+    rewrite/map12d/= !FmapE.fmapE not_fnd// !simpl_set.
+    by rewrite !eqxx/= !fsetU0.
+  Qed.
+
+  Lemma rename_app fv f a v:
+    (rename fv (Tm_App f a) v).2 = 
+    app
+      (ren
+      (fresh_tm (fresh_tm (vars f `|` vars a `|` fv) v f).1
+      (fresh_tm (vars f `|` vars a `|` fv) v f).2 a).2 f)
+      (ren
+      (fresh_tm (fresh_tm (vars f `|` vars a `|` fv) v f).1
+      (fresh_tm (vars f `|` vars a `|` fv) v f).2 a).2 a).
+  Proof. by rewrite/rename/= !push/=. Qed.
 
   Goal exists f s, runT u p' fset0 fmap0 (TA (call map12d)) (One s) false f /\ deref s X = list24.
   Proof.
@@ -340,29 +327,58 @@ Section map.
     split.
       apply: StepT'=> //=; cycle 1.
       rewrite/bc ifF ?acyclic_sigma0//.
-      rewrite p'map.
-      set s0 := (_ `|` _).
+      rewrite !simpl_set.
       rewrite !fresh_rules_cons !fstS !sndS.
       rewrite !simpl_set.
       set F0 := (_ `|` _).
       set F1 := (_ `|` _).
       set F2 := (_ `|` _).
       rewrite select_consF// [head _]/=.
-      rewrite [flatten_term (Tm_App _ _)]/= [flatten_mode _]/=.
-      rewrite fmapIn; last by rewrite !inE.
-      rewrite [odflt _ _]/=.
-      replace (H _ _ _ _ _ _) with (@None Sigma); last first.
-        rewrite/= !simpl_set /matching/montanari_deref deref_empty/=.
-        rewrite{2}/montanari_pair montanari_equation/=.
-        rewrite montanari_equation/=/montanari_pair.
+      rewrite get_input_vars_map12d fmapIn?inE//.
+      case H: H => //.
+        exfalso; move: H; rewrite/map12d/H eqxx !FmapE.fmapE.
+        rewrite eqxx [omap _ _]/= /mapS [omap _ _]/=.
+        case M: matching => //.
+        rewrite [omap _ _]/=.
+        cbn match.
+        rewrite eqxx [omap _ _]/=.
+        rewrite/matching/montanari_deref/montanari_pair.
+        rewrite !ground_deref//; last first.
+          by rewrite/list12/ground/= !simpl_set.
         by rewrite montanari_equation/=.
-      rewrite select_consF//head_fresh_rule [head _]/= /rename (push (fresh_tm _ _ _)) sndS; last by [].
+      rewrite {H} select_consF.
+      rewrite head_fresh_rule [head _]/=.
+      rewrite get_input_vars_map12d/map12d premises_fresh_rule [head _]/=.
+      rewrite [vars _]/= !simpl_set [premises _]/=.
       set F3 := (_ `|` _).
-
-      rewrite/fresh_tm !simpl_set.
-      rewrite !inE.
-      set F4 := _ `|` _.
-      set F5 := _ `|` _.
-      set F6 := _ `|` _.
-  Abort. *)
+      rewrite !rename_app !ren_app !ren_P.
+      rewrite [vars _]/= !simpl_set [vars _]/= !simpl_set.
+      set FT := (fresh_tm _ _ _).2.
+      rewrite/H eqxx !FmapE.fmapE eqxx [omap _ _]/= /mapS eqxx.
+      rewrite/u [lang.matching _]/=.
+      rewrite/matching/montanari_deref/montanari_pair.
+      rewrite !deref_empty montanari_equation [omap _ _]/=.
+      rewrite montanari_equation [omap _ _]/=.
+      cbn match; rewrite eqxx.
+      rewrite in_fnd.
+        apply/fsubsetP.
+          apply: fresh_tm_domf_sub.
+        apply/fsubsetP.
+          apply: fresh_tm_sub1.
+        by rewrite/= !inE eqxx.
+      move=> iFT; rewrite !deref_App !odflt_Some !deref_P.
+      rewrite deref_sigma0 not_in_deref; last first.
+        rewrite/= fsetU0 fdisjointX1 inE.
+        admit.
+      rewrite not_in_deref; last first.
+        admit.
+      rewrite 3!montanari_equation.
+      case: eqP => [H|_].
+        by exfalso; move: H; rewrite/ren; case: fndP => //.
+      case: eqP => [H|_].
+        by exfalso; move: H; rewrite/ren; case: fndP => //.
+      rewrite montanari_equation eqxx montanari_equation.
+      case: eqP => [H|_].
+        by exfalso; move: H; rewrite/ren; case: fndP => //.
+  Abort.
 End map.
